eve/Src/framework/eiffel2boogie/tasks/e2b_merge_results_task.e
@@ -15,11 +15,11 @@ create
 
 feature {NONE} -- Initialization
 
-	make (a_initial_result: attached like initial_result; a_secondary_verifier: attached like secondary_verifier)
+	make (a_initial_result: attached like initial_result; a_secondary_result_generator: attached like secondary_result_generator)
 			-- Initialize task.
 		do
 			initial_result := a_initial_result
-			secondary_verifier := a_secondary_verifier
+			secondary_result_generator := a_secondary_result_generator
 			has_next_step := True
 		end
 
@@ -41,42 +41,41 @@ feature {ROTA_S, ROTA_TASK_I} -- Basic operations
 		do
 			if
 				attached initial_result and then
-				attached secondary_verifier.last_result
+				attached secondary_result_generator.last_result
 			then
-				across secondary_verifier.last_result.procedure_results as l_second_results loop
-					if attached {E2B_SUCCESSFUL_VERIFICATION} l_second_results.item as l_second_success then
-						from
-							l_new_success := True
-							initial_result.verification_results.start
-						until
-							initial_result.verification_results.after or not l_new_success
-						loop
-							l_primary_result := initial_result.verification_results.item
-							if
-								l_primary_result.context_class.class_id = l_second_success.context_class.class_id and then
-								l_primary_result.context_feature.body_index = l_second_success.context_feature.body_index
-							then
-								if attached {E2B_SUCCESSFUL_VERIFICATION} l_primary_result then
-									l_new_success := False
-								elseif attached {E2B_FAILED_VERIFICATION} l_primary_result as l_primary_failed then
-									across l_primary_failed.errors as l_errors loop
-										l_second_success.add_original_error (l_errors.item)
-									end
-									initial_result.verification_results.remove
-								elseif attached {E2B_INCONCLUSIVE_RESULT} l_primary_result then
-										-- Ignore
-								else
-									check internal_error: False end
+				across secondary_result_generator.last_result.successful_verifications as l_second_success loop
+					from
+						l_new_success := True
+						initial_result.verification_results.start
+					until
+						initial_result.verification_results.after or not l_new_success
+					loop
+						l_primary_result := initial_result.verification_results.item
+						if
+							l_primary_result.context_class.class_id = l_second_success.item.context_class.class_id and then
+							l_primary_result.context_feature.body_index = l_second_success.item.context_feature.body_index
+						then
+							if attached {E2B_SUCCESSFUL_VERIFICATION} l_primary_result then
+								l_new_success := False
+							elseif attached {E2B_FAILED_VERIFICATION} l_primary_result as l_primary_failed then
+								across l_primary_failed.errors as l_errors loop
+									l_second_success.item.add_original_error (l_errors.item)
 								end
+								initial_result.verification_results.remove
+							elseif attached {E2B_INCONCLUSIVE_RESULT} l_primary_result then
+									-- Ignore
 							else
-								initial_result.verification_results.forth
+								check internal_error: False end
 							end
-						end
-						if l_new_success then
-							initial_result.verification_results.extend (l_second_success)
+						else
+							initial_result.verification_results.forth
 						end
 					end
+					if l_new_success then
+						initial_result.verification_results.extend (l_second_success.item)
+					end
 				end
+
 			end
 			has_next_step := False
 		end
@@ -92,7 +91,7 @@ feature {NONE} -- Implementation
 	initial_result: attached E2B_RESULT
 			-- Initial result.
 
-	secondary_verifier: attached E2B_VERIFIER
-			-- Boogie verifier.
+	secondary_result_generator: attached E2B_RESULT_GENERATOR
+			-- Boogie result generator.
 
 end
