eve/Src/framework/eiffel2boogie/tasks/e2b_verify_with_inlining_task.e
@@ -10,6 +10,8 @@ inherit
 
 	ROTA_TASK_I
 
+	E2B_SHARED_CONTEXT
+
 create
 	make
 
@@ -54,6 +56,12 @@ feature {ROTA_S, ROTA_TASK_I} -- Basic operations
 				end
 
 				create l_boogie_universe.make
+				boogie_universe_cell.put (l_boogie_universe)
+				helper.reset
+				translation_pool.reset
+				autoproof_errors.wipe_out
+				result_handlers.wipe_out
+
 				create inlining_verifier.make
 				create result_generator.make
 				remaining_tasks.start
@@ -62,7 +70,7 @@ feature {ROTA_S, ROTA_TASK_I} -- Basic operations
 				remaining_tasks.put_left (create {E2B_GENERATE_BOOGIE_TASK}.make (l_boogie_universe, inlining_verifier))
 				remaining_tasks.put_left (create {E2B_EXECUTE_BOOGIE_TASK}.make (inlining_verifier))
 				remaining_tasks.put_left (create {E2B_EVALUATE_BOOGIE_OUTPUT_TASK}.make (inlining_verifier, result_generator))
-				remaining_tasks.put_left (create {E2B_MERGE_RESULTS_TASK}.make (initial_result_generator.last_result, inlining_verifier))
+				remaining_tasks.put_left (create {E2B_MERGE_RESULTS_TASK}.make (initial_result_generator.last_result, result_generator))
 			end
 			has_next_step := False
 		end
